Remove unnecessary starting iterator from VMPath as it cannot be constrained by outside.

correctness/RegexCorrectness/VM/Path/VMPath.lean
@@ -11,25 +11,25 @@ open String (Pos Iterator)
 
 namespace Regex.NFA
 
-inductive VMPath (nfa : NFA) (wf : nfa.WellFormed) (it : Iterator) : Iterator → Fin nfa.nodes.size → List (Nat × Pos) → Prop where
-  | init {i update} (cls : nfa.εClosure' it ⟨nfa.start, wf.start_lt⟩ i update) :
-    VMPath nfa wf it it i update
-  | more {i j k it' update₁ update₂} (prev : VMPath nfa wf it it' i update₁) (step : nfa.CharStep it' i j) (cls : nfa.εClosure' it'.next j k update₂) :
-    VMPath nfa wf it it'.next k (update₁ ++ update₂)
+inductive VMPath (nfa : NFA) (wf : nfa.WellFormed) : Iterator → Fin nfa.nodes.size → List (Nat × Pos) → Prop where
+  | init {it i update} (cls : nfa.εClosure' it ⟨nfa.start, wf.start_lt⟩ i update) :
+    VMPath nfa wf it i update
+  | more {i j k it update₁ update₂} (prev : VMPath nfa wf it i update₁) (step : nfa.CharStep it i j) (cls : nfa.εClosure' it.next j k update₂) :
+    VMPath nfa wf it.next k (update₁ ++ update₂)
 
 namespace VMPath
 
-theorem eq_or_nfaPath {nfa : NFA} {wf it it' i update} (path : nfa.VMPath wf it it' i update) :
-  (it' = it ∧ i.val = nfa.start ∧ update = []) ∨
-  nfa.Path 0 nfa.start it i it' update := by
+theorem eq_or_nfaPath {nfa : NFA} {wf it i update} (path : nfa.VMPath wf it i update) :
+  (i.val = nfa.start ∧ update = []) ∨
+  ∃ it₀, nfa.Path 0 nfa.start it₀ i it update := by
   induction path with
-  | @init i update cls =>
+  | @init it i update cls =>
     simp [εClosure'_iff_path nfa wf] at cls
     cases cls with
     | inl h => simp [←h.1, h.2]
-    | inr cls => exact .inr cls
-  | @more i j k it' update₁ update₂ prev step cls ih =>
-    have path₂ : nfa.Path 0 i it' k it'.next update₂ := by
+    | inr cls => exact .inr ⟨it, cls⟩
+  | @more i j k it update₁ update₂ prev step cls ih =>
+    have path₂ : nfa.Path 0 i it k it.next update₂ := by
       simp [εClosure'_iff_path nfa wf] at cls
       match cls with
       | .inl ⟨eqk, equpdate, v⟩ =>
@@ -38,14 +38,14 @@ theorem eq_or_nfaPath {nfa : NFA} {wf it it' i update} (path : nfa.VMPath wf it 
       | .inr path => exact .more step path
 
     match ih with
-    | .inl ⟨eqit, eqi, equpdate⟩ =>
-      simp [←eqit, ←eqi, equpdate]
-      exact path₂
-    | .inr path₁ => exact .inr (path₁.trans path₂)
+    | .inl ⟨eqi, equpdate⟩ =>
+      simp [←eqi, equpdate]
+      exact .inr ⟨it, path₂⟩
+    | .inr ⟨it₀, path₁⟩ => exact .inr ⟨it₀, path₁.trans path₂⟩
 
-theorem nfaPath_of_ne {nfa : NFA} {wf it it' i update} (path : nfa.VMPath wf it it' i update)
+theorem nfaPath_of_ne {nfa : NFA} {wf it i update} (path : nfa.VMPath wf it i update)
   (ne : i.val ≠ nfa.start):
-  nfa.Path 0 nfa.start it i it' update := by
+  ∃ it₀, nfa.Path 0 nfa.start it₀ i it update := by
   simpa [ne] using eq_or_nfaPath path
 
 end VMPath
@@ -65,13 +65,11 @@ def WriteUpdate {nfa : NFA} (i : Fin nfa.nodes.size) : Prop :=
 /--
 All states in `next.state` have a corresponding path from `nfa.start` to the state where the span
 ends at `it`, and their updates are written to `next.updates` when necessary.
-
-TODO: I don't understand how this should be updated for Iterators.
 -/
 def SearchState.Inv (nfa : NFA) (wf : nfa.WellFormed) (it : Iterator) (next : SearchState HistoryStrategy nfa) : Prop :=
   ∀ i ∈ next.states,
-    ∃ it₀ update,
-      nfa.VMPath wf it₀ it i update ∧
+    ∃ update,
+      nfa.VMPath wf it i update ∧
       (WriteUpdate i → next.updates[i] = update)
 
 theorem SearchState.Inv.of_empty {nfa wf it} {next : SearchState HistoryStrategy nfa} (h : next.states.isEmpty) :
