correctness/RegexCorrectness/VM/Search/Compile.lean
@@ -16,13 +16,13 @@ theorem captures_of_captureNext_some {e nfa it₀ matched'} (eq : NFA.compile e 
     it'.toString = it₀.toString ∧
     e.Captures it it' groups ∧
     EquivUpdate groups (matched'.get isSome') := by
-  have ⟨state, it, it', eqstring, hn, path⟩ := captureNext.path_done_of_matched h v isSome'
+  have ⟨state, it', eqstring, hn, path⟩ := captureNext.path_done_of_matched h v isSome'
   have eq_zero := (NFA.done_iff_zero_compile eq state).mp hn
   have : state.val ≠ nfa.start := by
     simp [eq_zero]
     have : 0 < nfa.start := NFA.lt_zero_start_compile eq
     exact Nat.ne_of_lt this
-  have path := path.nfaPath_of_ne this
+  have ⟨it, path⟩ := path.nfaPath_of_ne this
   simp [eq_zero] at path
   have ⟨groups, eqv, c⟩ := NFA.captures_of_path_compile eq (path.compile_liftBound eq)
   exact ⟨it, it', groups, eqstring, c, eqv⟩
